ulib/FStar.Pervasives.fst
@@ -358,15 +358,5 @@ unopteq type dtuple8 (a:Type)
 val ignore: #a:Type -> a -> Tot unit
 let ignore #a x = ()
 
-
-(*********************************************************************************)
-(* Marking terms for normalization *)
-(*********************************************************************************)
-abstract let normalize_term (#a:Type) (x:a) : a = x
-abstract let normalize (a:Type0) = a
-
-val assert_norm : p:Type -> Pure unit (requires (normalize p)) (ensures (fun _ -> p))
-let assert_norm p = ()
-
 val false_elim : #a:Type -> u:unit{false} -> Tot a
 let rec false_elim #a u = false_elim ()
