ulib/prims.fst
@@ -316,3 +316,14 @@ let abs (x:int) : Tot int = if x >= 0 then x else -x
 
 assume val string_of_bool: bool -> Tot string
 assume val string_of_int: int -> Tot string
+
+
+
+(*********************************************************************************)
+(* Marking terms for normalization *)
+(*********************************************************************************)
+abstract let normalize_term (#a:Type) (x:a) : a = x
+abstract let normalize (a:Type0) = a
+
+val assert_norm : p:Type -> Pure unit (requires (normalize p)) (ensures (fun _ -> p))
+let assert_norm p = ()
